src/lib/data/Kuiper.Matrix4.fsti
@@ -89,6 +89,7 @@ instance has_pts_to
 }
 
 inline_for_extraction noextract
+ghost
 fn gpu_matrix_concr
   (#et:Type)
   (#mrows #mcols #brows #bcols : erased nat)
@@ -103,19 +104,16 @@ fn gpu_matrix_concr
 inline_for_extraction noextract
 fn gpu_matrix_abs
   (#et:Type)
-  (#mrows0 #brows0 #mcols0 #bcols0 : erased nat)
-  (#l0 : mlayout4 mrows0 brows0 mcols0 bcols0)
-  (g : gpu_matrix et l0)
   (#mrows #mcols #brows #bcols : erased nat)
   (l : mlayout4 mrows mcols brows bcols)
+  (p : gpu_array et (mlayout_size l))
   (#em : ematrix4 et mrows mcols brows bcols)
   requires
-    core g |-> to_seq l em
+    p |-> to_seq l em
   returns
     g' : gpu_matrix et l
   ensures
-    pure (mlayout_size l == mlayout_size l0 /\
-          core g == core g') **
+    pure (core g' == p) **
     (g' |-> em)
 
 inline_for_extraction noextract
